more refactor

src/examples/matmul-tile-f32/Kuiper.MatMulTileF32.Prep.fst
@@ -8,9 +8,11 @@ open Kuiper.Math
 
 module A    = Pulse.Lib.Array
 module SZ   = FStar.SizeT
-module Defs = Kuiper.MatMul.Defs
-module Kernel = Kuiper.MatMulTileF32.Kernel
 module Barrier = Kuiper.MatMulTileF32.Barrier
+
+module P = Kuiper.MatMul.Pure
+module I = Kuiper.MatMul.Impure
+module K = Kuiper.MatMulTileF32.Kernel
 
 let lemma_nonneg_mul (x y : int)
   : Lemma (requires x >= 0 /\ y >= 0)
@@ -37,14 +39,14 @@ fn setup
            gpu_pts_to_array ga1 v1 **
            gpu_pts_to_array ga2 v2
   ensures  bigstar 0 (nblk * nthr) (fun i ->
-             Kernel.kpre rows shared columns ga1 ga2 gr #v1 #v2 (nblk * nthr)
-               (Kernel.tid_to_idx rows shared columns bdim i))
+             K.kpre rows shared columns ga1 ga2 gr #v1 #v2 (nblk * nthr)
+               (K.tid_to_idx rows shared columns bdim i))
 {
   // Sharing the input matrices (splitting permissions)
-  fold Defs.gpu_pts_to_matrix rows   shared  ga1 1 v1;
-  fold Defs.gpu_pts_to_matrix shared columns ga2 1 v2;
-  Defs.gpu_matrix_share_underspec #_ #1 rows   shared  ga1 (nblk * nthr) v1;
-  Defs.gpu_matrix_share_underspec #_ #2 shared columns ga2 (nblk * nthr) v2;
+  fold I.gpu_pts_to_matrix rows   shared  ga1 1 v1;
+  fold I.gpu_pts_to_matrix shared columns ga2 1 v2;
+  I.gpu_matrix_share_underspec #_ #1 rows   shared  ga1 (nblk * nthr) v1;
+  I.gpu_matrix_share_underspec #_ #2 shared columns ga2 (nblk * nthr) v2;
 
   // Sharing the output matrix (splitting each cell)
   gpu_pts_to_ref gr; (* obtain length v == (nblk * nthr) *)
@@ -58,11 +60,11 @@ fn setup
   ghost
   fn aux (i:nat{0 <= i /\ i < (nblk * nthr)})
     requires
-      Defs.gpu_pts_to_matrix rows   shared  ga1 (nblk * nthr) v1 **
-      Defs.gpu_pts_to_matrix shared columns ga2 (nblk * nthr) v2 **
+      I.gpu_pts_to_matrix rows   shared  ga1 (nblk * nthr) v1 **
+      I.gpu_pts_to_matrix shared columns ga2 (nblk * nthr) v2 **
       gpu_pts_to_array_slice gr i (i + 1) seq![s `Seq.index` i]
     ensures
-      Kernel.kpre rows shared columns ga1 ga2 gr #v1 #v2 (nblk * nthr) i
+      K.kpre rows shared columns ga1 ga2 gr #v1 #v2 (nblk * nthr) i
   {
     fold gpu_pts_to_array1 gr i;
     ()
@@ -78,10 +80,10 @@ fn setup
   lemma_divides_exact columns bdim;
   assert (pure (rows / bdim >= 1));
   assert (pure (columns / bdim >= 1));
-  bigstar_permute #0 #0 #(nblk * nthr) #_ (Kernel.permute (rows/bdim) (columns/bdim) bdim);
+  bigstar_permute #0 #0 #(nblk * nthr) #_ (K.permute (rows/bdim) (columns/bdim) bdim);
   ghost fn rewrite_permute_to_fn (i: nat {0 <= i /\ i < (nblk * nthr)})
-    requires Kernel.kpre rows shared columns ga1 ga2 gr #v1 #v2 (nblk * nthr) ((Kernel.permute (rows/bdim) (columns/bdim) bdim).f i)
-    ensures  Kernel.kpre rows shared columns ga1 ga2 gr #v1 #v2 (nblk * nthr) (Kernel.tid_to_idx rows shared columns bdim i)
+    requires K.kpre rows shared columns ga1 ga2 gr #v1 #v2 (nblk * nthr) ((K.permute (rows/bdim) (columns/bdim) bdim).f i)
+    ensures  K.kpre rows shared columns ga1 ga2 gr #v1 #v2 (nblk * nthr) (K.tid_to_idx rows shared columns bdim i)
   {
     ()
   };
@@ -106,7 +108,7 @@ fn breakdown
   (v2 : seq f32 { Seq.length v2 == shared * columns })
   requires
     bigstar 0 (nblk * nthr) (fun i ->
-      Kernel.kpost rows shared columns ga1 ga2 gr #v1 #v2 (nblk * nthr) (Kernel.tid_to_idx rows shared columns bdim i))
+      K.kpost rows shared columns ga1 ga2 gr #v1 #v2 (nblk * nthr) (K.tid_to_idx rows shared columns bdim i))
   ensures
     (exists* vr. gpu_pts_to_array gr vr) **
     gpu_pts_to_array ga1 v1 **
@@ -122,20 +124,20 @@ fn breakdown
   };
   assert (pure (rows / bdim >= 1));
   assert (pure (columns / bdim >= 1));
-  let perm = perm_inv (Kernel.permute (rows/bdim) (columns/bdim) bdim);
+  let perm = perm_inv (K.permute (rows/bdim) (columns/bdim) bdim);
   bigstar_permute #0 #0 #(nblk * nthr) #_ perm;
   ghost fn rewrite_permute_to_fn (i: nat {0 <= i /\ i < (nblk * nthr)})
-    requires Kernel.kpost rows shared columns ga1 ga2 gr #v1 #v2 (nblk * nthr) (perm.f (Kernel.tid_to_idx rows shared columns bdim i))
-    ensures  Kernel.kpost rows shared columns ga1 ga2 gr #v1 #v2 (nblk * nthr) i
+    requires K.kpost rows shared columns ga1 ga2 gr #v1 #v2 (nblk * nthr) (perm.f (K.tid_to_idx rows shared columns bdim i))
+    ensures  K.kpost rows shared columns ga1 ga2 gr #v1 #v2 (nblk * nthr) i
   {
-    let once: (j: nat{ 0 <= j /\ j < (nblk * nthr) }) = Kernel.tid_to_idx rows shared columns bdim i;
+    let once: (j: nat{ 0 <= j /\ j < (nblk * nthr) }) = K.tid_to_idx rows shared columns bdim i;
     let once': (j: nat{ 0 <= j /\ j < (nblk * nthr) }) = perm.g i;
     assert (pure (once' == once));
     perm.proof once i;
     // f x == y <==> g y == x
     let double: (j: nat{ 0 <= j /\ j < (nblk * nthr) }) = perm.f once;
     assert (pure (double == i));
-    rewrite (gpu_pts_to_array1 gr (perm.f (Kernel.tid_to_idx rows shared columns bdim i)))
+    rewrite (gpu_pts_to_array1 gr (perm.f (K.tid_to_idx rows shared columns bdim i)))
          as (gpu_pts_to_array1 gr i);
     ()
   };
@@ -149,10 +151,10 @@ fn breakdown
   gpu_array_unslice_1_underspec #4 gr #1.0R;
 
   // Unsharing the input matrices (gathering permissions)
-  Defs.gpu_matrix_unshare_underspec #_ #1 rows   shared  ga1 (nblk * nthr) v1;
-  Defs.gpu_matrix_unshare_underspec #_ #2 shared columns ga2 (nblk * nthr) v2;
-  unfold Defs.gpu_pts_to_matrix rows   shared  ga1 1 v1;
-  unfold Defs.gpu_pts_to_matrix shared columns ga2 1 v2;
+  I.gpu_matrix_unshare_underspec #_ #1 rows   shared  ga1 (nblk * nthr) v1;
+  I.gpu_matrix_unshare_underspec #_ #2 shared columns ga2 (nblk * nthr) v2;
+  unfold I.gpu_pts_to_matrix rows   shared  ga1 1 v1;
+  unfold I.gpu_pts_to_matrix shared columns ga2 1 v2;
 
   ()
 }
